Common/Exceptions.thy
@@ -1,12 +1,9 @@
-(*  Title:      HOL/MicroJava/J/Exceptions.thy
+(*  Title:      JinjaDCI/Common/Exceptions.thy
 
-    Author:     Gerwin Klein, Martin Strecker
-    Copyright   2002 Technische Universitaet Muenchen
-*)
-(*
-  Expanded to include more error types in support of statics and dynamic class initialization.
-  Susannah Mansky
-  2016-17, UIUC
+    Author:     Gerwin Klein, Martin Strecker, Susannah Mansky
+    Copyright   2002 Technische Universitaet Muenchen, 2019-20 UIUC
+
+    Based on the Jinja theory Common/Exceptions.thy by Gerwin Klein and Martin Strecker
 *)
 
 section \<open> Exceptions \<close>
@@ -66,16 +63,19 @@ lemmas sys_xcpts_defs = NullPointer_def ClassCast_def OutOfMemory_def NoClassDef
 
 lemma Start_nsys_xcpts: "Start \<notin> sys_xcpts"
  by(simp add: Start_def sys_xcpts_def sys_xcpts_defs)
-lemma [simp]: "Start \<noteq> NullPointer" "Start \<noteq> ClassCast" "Start \<noteq> OutOfMemory"
- "Start \<noteq> NoClassDefFoundError" "Start \<noteq> IncompatibleClassChangeError"
- "Start \<noteq> NoSuchFieldError" "Start \<noteq> NoSuchMethodError"
+
+lemma Start_nsys_xcpts1 [simp]: "Start \<noteq> NullPointer" "Start \<noteq> ClassCast"
+ "Start \<noteq> OutOfMemory" "Start \<noteq> NoClassDefFoundError"
+ "Start \<noteq> IncompatibleClassChangeError" "Start \<noteq> NoSuchFieldError"
+ "Start \<noteq> NoSuchMethodError"
 using Start_nsys_xcpts by(auto simp: sys_xcpts_def)
-lemma [simp]: "NullPointer \<noteq> Start" "ClassCast \<noteq> Start" "OutOfMemory \<noteq> Start"
- "NoClassDefFoundError \<noteq> Start" "IncompatibleClassChangeError \<noteq> Start"
- "NoSuchFieldError \<noteq> Start" "NoSuchMethodError \<noteq> Start"
+
+lemma Start_nsys_xcpts2 [simp]: "NullPointer \<noteq> Start" "ClassCast \<noteq> Start"
+ "OutOfMemory \<noteq> Start" "NoClassDefFoundError \<noteq> Start"
+ "IncompatibleClassChangeError \<noteq> Start" "NoSuchFieldError \<noteq> Start"
+ "NoSuchMethodError \<noteq> Start"
 using Start_nsys_xcpts by(auto simp: sys_xcpts_def dest: sym)
 
-(* pre-linked version *)
 definition start_heap :: "'c prog \<Rightarrow> heap"
 where
   "start_heap G \<equiv> Map.empty (addr_of_sys_xcpt NullPointer \<mapsto> blank G NullPointer)
@@ -92,12 +92,11 @@ where
 
 subsection "System exceptions"
 
-lemma [simp]: "NullPointer \<in> sys_xcpts \<and> OutOfMemory \<in> sys_xcpts \<and> ClassCast \<in> sys_xcpts
-   \<and> NoClassDefFoundError \<in> sys_xcpts
+lemma sys_xcpts_incl [simp]: "NullPointer \<in> sys_xcpts \<and> OutOfMemory \<in> sys_xcpts
+   \<and> ClassCast \<in> sys_xcpts \<and> NoClassDefFoundError \<in> sys_xcpts
    \<and> IncompatibleClassChangeError \<in> sys_xcpts \<and> NoSuchFieldError \<in> sys_xcpts
    \<and> NoSuchMethodError \<in> sys_xcpts"
 (*<*)by(simp add: sys_xcpts_def)(*>*)
-
 
 lemma sys_xcpts_cases [consumes 1, cases set]:
   "\<lbrakk> C \<in> sys_xcpts; P NullPointer; P OutOfMemory; P ClassCast; P NoClassDefFoundError;
@@ -105,12 +104,20 @@ lemma sys_xcpts_cases [consumes 1, cases set]:
   P NoSuchMethodError \<rbrakk> \<Longrightarrow> P C"
 (*<*)by (auto simp: sys_xcpts_def)(*>*)
 
+subsection "Starting heap"
+
 lemma start_heap_sys_xcpts:
 assumes "C \<in> sys_xcpts"
 shows "start_heap P (addr_of_sys_xcpt C) = Some(blank P C)"
-apply(rule sys_xcpts_cases[OF assms])
-      apply(auto simp add: start_heap_def sys_xcpts_def addr_of_sys_xcpt_def sys_xcpts_defs)
-done
+by(rule sys_xcpts_cases[OF assms])
+  (auto simp add: start_heap_def sys_xcpts_def addr_of_sys_xcpt_def sys_xcpts_defs)
+
+lemma start_heap_classes:
+ "start_heap P a = Some(C,fs) \<Longrightarrow> C \<in> sys_xcpts"
+ by(simp add: start_heap_def blank_def split: if_split_asm)
+
+lemma start_heap_nStart: "start_heap P a = Some obj \<Longrightarrow> fst(obj) \<noteq> Start"
+ by(cases obj, auto dest!: start_heap_classes simp: Start_nsys_xcpts)
 
 subsection "@{term preallocated}"
 
@@ -177,12 +184,5 @@ lemmas preallocated_new  = preallocated_hext [OF _ hext_new]
 lemma preallocated_start:
   "preallocated (start_heap P)"
  by(auto simp: start_heap_sys_xcpts blank_def preallocated_def)
-
-lemma start_heap_classes:
- "start_heap P a = Some(C,fs) \<Longrightarrow> C \<in> sys_xcpts"
- by(simp add: start_heap_def blank_def split: if_split_asm)
-
-lemma start_heap_nStart: "start_heap P a = Some obj \<Longrightarrow> fst(obj) \<noteq> Start"
- by(cases obj, auto dest!: start_heap_classes simp: Start_nsys_xcpts)
 
 end
