JinjaDCI.thy
@@ -2,15 +2,9 @@ theory JinjaDCI
 imports
   "J/Equivalence"
   "J/Annotate"
-  (* FIXME "Example" *)
-(* "J/execute_Bigstep"
-  "J/execute_WellType" *)
-(*  "JVM/JVMDefensive" *)
-(*  "JVM/JVMListExample" *)
-(*  "BV/BVExec" *)
-(*  "BV/LBVJVM" *) "BV/TF_JVM"
-   "BV/BVNoTypeError"
-(*  "BV/BVExample" *)
+  "JVM/JVMDefensive"
+  "BV/TF_JVM"
+  "BV/BVNoTypeError"
   "Compiler/TypeComp"
 begin
 
